src/lib/poly/gemm/Kuiper.Poly.GEMM.BlockTiling2D.fst
@@ -5,6 +5,7 @@ module Kuiper.Poly.GEMM.BlockTiling2D
 #set-options "--z3rlimit 60"
 
 open Kuiper
+open Kuiper.Approximates
 open Kuiper.Array.Vectorized { has_vec_cpy, chunk }
 open Kuiper.EMatrix { ematrix }
 open Kuiper.Math { even, odd, even_2x, odd_2x1 }
@@ -19,6 +20,8 @@ module B = Kuiper.Barrier
 module MS = Kuiper.Spec.GEMM
 module SZ = Kuiper.SizeT
 module FB = Kuiper.Poly.GEMM.FlipFlopBarrier
+
+module MU = Kuiper.Poly.GEMM.Util
 
 inline_for_extraction noextract
 let ttile
@@ -1393,7 +1396,7 @@ let mk_kernel
 #pop-options
 
 inline_for_extraction noextract
-fn mmcomb_gpu
+fn mmcomb_gpu_exact
   (#et : Type0) {| scalar et, has_vec_cpy et |}
   (comb : binop et)
   (#rows #shared #cols : szp)
@@ -1443,4 +1446,65 @@ fn mmcomb_gpu
 {
   (* fixed the inner layouts, or we'd have to propagate this everywhere? *)
   launch_sync (mk_kernel comb gA gB gC bm bn bk slA slB tm tn (rows/^bm *^ (cols/^bn)) (bm/^tm *^ (bn/^tn)) ());
+}
+
+inline_for_extraction noextract
+fn mmcomb_gpu_approx
+  (#et : Type0) {| scalar et, has_vec_cpy et, real_like et |}
+  (comb : binop et)
+  (comb_r : binop real { approx2 comb comb_r })
+  (#rows #shared #cols : szp)
+  (#lA : mlayout rows shared)
+  (#lB : mlayout shared cols)
+  (#lC : mlayout rows cols)
+  {| clayout lA, clayout lB, clayout lC |}
+  {| str_A : strided_row_major lA,
+     str_B : strided_row_major lB |}
+  (#_ : squash (aligned_strided_row_major (chunk et) str_A))
+  (#_ : squash (aligned_strided_row_major (chunk et) str_B))
+  (gA : gpu_matrix et lA { is_global_matrix gA })
+  (#eA : ematrix et rows shared)
+  (gB : gpu_matrix et lB { is_global_matrix gB })
+  (#eB : ematrix et shared cols)
+  (gC : gpu_matrix et lC { is_global_matrix gC })
+  (#eC : ematrix et rows cols)
+  (bm : szp{bm /?+ rows})
+  (bn : szp{bn /?+ cols})
+  (bk : szp{bk /?+ shared})
+  (#_ : squash (chunk et /?+ bn))
+  (#_ : squash (chunk et /?+ bk))
+  (tm : szp{tm /?+ bm})
+  (tn : szp{tn /?+ bn})
+  (#_ : squash (chunk et * (bm/tm * (bn/tn)) /?+ (bm * bk)))
+  (#_ : squash (chunk et * (bm/tm * (bn/tn)) /?+ (bk * bn)))
+  (#_ : squash (SZ.fits (bm*bk + bm/tm*(bn/tn))))
+  (#_ : squash (SZ.fits (bk*bn + bm/tm*(bn/tn))))
+  (#_: squash (SZ.fits (bm * bk) /\ SZ.fits (bk * bn)))
+  (slA : full_mlayout bm bk)
+  (slB : full_mlayout bk bn)
+  {| clayout slA, clayout slB |}
+  (#fA #fB : perm)
+  (rA : ematrix real rows shared)
+  (rB : ematrix real shared cols)
+  (rC : ematrix real rows cols)
+  norewrite
+  preserves
+    cpu **
+    on gpu_loc (gA |-> Frac fA eA) **
+    on gpu_loc (gB |-> Frac fB eB)
+  requires
+    pure (aligned 16 (core gA)) **
+    pure (aligned 16 (core gB)) **
+    pure (rows/bm * (cols/bn) <= max_blocks) **
+    pure (bm/tm * (bn/tn) <= max_threads) **
+    pure (eA %~ rA /\ eB %~ rB /\ eC %~ rC) **
+    on gpu_loc (gC |-> eC)
+  ensures
+    exists* (eC' : ematrix et rows cols).
+      on gpu_loc (gC |-> eC') **
+      pure (eC' %~ MS.mmcomb comb_r rC rA rB)
+{
+  mmcomb_gpu_exact #et #_ #_ comb #rows #shared #cols #lA #lB #lC gA #eA gB #eB gC #eC bm bn bk tm tn slA slB #_ #_;
+  MU.mmcomb_approx_real comb comb_r eC eA eB rA rB rC;
+  ()
 }
